module Lib.Nat where

open import Lib.Zero using (ğŸ˜; Â¬_)
open import Lib.One using (ğŸ™)
open import Project.Control.Equality using (_â‰¡_; refl; sym; cong; cong-app; trans; subst; â‰¡-equiv)
open import Project.EquationalReasoning as EquationalReasoning
open module â‰¡-Reasoning {n} {A} =
       EquationalReasoning.Core {n} {A} _â‰¡_ {{â‰¡-equiv}}
         using (begin_; _âˆ¼âŸ¨âŸ©_; step-âˆ¼; _âˆ;
                reflexive; symmetric; transitive)

data â„• : Set where
  zero : â„•
  suc  : â„• â†’ â„•

{-# BUILTIN NATURAL â„• #-}

_+_ : â„• â†’ â„• â†’ â„•
zero  + m = m
suc n + m = suc (n + m)
infixr 100 _+_

{-# BUILTIN NATPLUS _+_ #-}

_<=_ : â„• â†’ â„• â†’ Set
zero  <= m     = ğŸ™
suc n <= zero  = ğŸ˜
suc n <= suc m = n <= m

_<_ : â„• â†’ â„• â†’ Set
n < m = suc n <= m

-- _*_  : â„• â†’ â„• â†’ â„•
-- zero * y = zero
-- suc x * y = y + (x * y)
-- infixr 120 _*_

---

+-assoc : (n m k : â„•) â†’ (n + m) + k â‰¡ n + (m + k)
+-assoc zero m k = refl
+-assoc (suc n) m k = cong suc (+-assoc n m k)

+-right-zero : (n : â„•) â†’ n + zero â‰¡ n
+-right-zero zero = refl
+-right-zero (suc n) =
  cong suc (+-right-zero n)

+-right-suc : (n m : â„•) â†’ suc (n + m) â‰¡ n + suc m
+-right-suc zero m = refl
+-right-suc (suc x) m = cong suc (+-right-suc x m)

+-commut : (n m : â„•) â†’ n + m â‰¡ m + n
+-commut zero m = symmetric (+-right-zero m)
+-commut (suc n) m
  rewrite +-commut n m
  rewrite +-right-suc m n =
  refl

data _â‰¤_ : â„• â†’ â„• â†’ Set where
  -- We know that zero is â‰¤ anything else
  ozero : {x : â„•} â†’ zero â‰¤ x
  -- We know that if x â‰¤ y, then suc x â‰¤ suc y also
  osuc : {x y : â„•} â†’ x â‰¤ y â†’ suc x â‰¤ suc y

infix 90 _â‰¤_

â‰¤-refl : (n : â„•) â†’ n â‰¤ n
â‰¤-refl zero = ozero
â‰¤-refl (suc x) = osuc (â‰¤-refl x)

â‰¤-suc : (n : â„•) â†’ n â‰¤ suc n
â‰¤-suc zero = ozero
â‰¤-suc (suc x) = osuc (â‰¤-suc x)

â‰¤-trans : {n m k : â„•} â†’ n â‰¤ m â†’ m â‰¤ k â†’ n â‰¤ k
â‰¤-trans ozero q = ozero
â‰¤-trans (osuc p) (osuc q) = osuc (â‰¤-trans p q)

â‰¤-antisymm : {n m : â„•} â†’ n â‰¤ m â†’ m â‰¤ n â†’ n â‰¡ m
â‰¤-antisymm ozero ozero = refl
â‰¤-antisymm (osuc p) (osuc q) = cong suc (â‰¤-antisymm p q)

â‰¤-refl-not-suc : {n : â„•} â†’ Â¬ (suc n â‰¤ n)
â‰¤-refl-not-suc (osuc sucnâ‰¤m) = â‰¤-refl-not-suc sucnâ‰¤m

â‰¤-suc-not-eq : {n m : â„•} â†’ suc n â‰¤ m â†’ Â¬ (n â‰¡ m)
â‰¤-suc-not-eq p refl = â‰¤-refl-not-suc p

â„•Eq : â„• â†’ â„• â†’ Set
â„•Eq zero zero = ğŸ™
â„•Eq zero (suc m) = ğŸ˜
â„•Eq (suc n) zero = ğŸ˜
â„•Eq (suc n) (suc m) = â„•Eq n m

_*_  : â„• â†’ â„• â†’ â„•
zero * m = zero
suc n * m = m + n * m
infixr 120 _*_

*-right-zero : (n : â„•) â†’ n * 0 â‰¡ 0
*-right-zero zero = refl
*-right-zero (suc n) = *-right-zero n

*-right-suc : (n m : â„•) â†’ n * suc m â‰¡ n + n * m
*-right-suc zero m = refl
*-right-suc (suc n) m rewrite *-right-suc n m = cong suc (
  begin
  m + n + n * m âˆ¼âŸ¨ symmetric (+-assoc m n (n * m)) âŸ©
  (m + n) + n * m âˆ¼âŸ¨ cong (_+ n * m) (+-commut m n) âŸ©
  (n + m) + n * m âˆ¼âŸ¨ +-assoc n m (n * m) âŸ©
  n + m + n * m
  âˆ)

*-commut : (n m : â„•) â†’ n * m â‰¡ m * n
*-commut zero m rewrite *-right-zero m = refl
*-commut (suc n) m =
  begin
    m + n * m
  âˆ¼âŸ¨ cong (m +_) (*-commut n m) âŸ©
    m + m * n
  âˆ¼âŸ¨ symmetric (*-right-suc m n) âŸ©
    m * suc n
  âˆ

*-left-distrib-+ : (n m k : â„•) â†’ n * (m + k) â‰¡ n * m + n * k
*-left-distrib-+ zero m k = refl
*-left-distrib-+ (suc n) m k =
  begin
    (m + k) + n * (m + k)
  âˆ¼âŸ¨ cong ((m + k) +_) (*-left-distrib-+ n m k) âŸ©
    (m + k) + (n * m + n * k)
  âˆ¼âŸ¨ +-assoc m k (n * m + n * k) âŸ©
    m + (k + ((n * m) + (n * k)))
  âˆ¼âŸ¨ cong (m +_) (symmetric (+-assoc k (n * m) (n * k))) âŸ©
    m + ((k + (n * m)) + (n * k))
  âˆ¼âŸ¨ cong (m +_) (cong-app (cong _+_ (+-commut k (n * m))) _) âŸ©
    m + (((n * m) + k) + (n * k))
  âˆ¼âŸ¨ cong (m +_) (+-assoc (n * m) k (n * k)) âŸ©
    m + ((n * m) + (k + (n * k)))
  âˆ¼âŸ¨ symmetric (+-assoc m (n * m) (k + n * k)) âŸ©
    (m + n * m) + (k + n * k)
  âˆ

*-right-distrib-+ : (n m k : â„•) â†’ (n + m) * k â‰¡ n * k + m * k
*-right-distrib-+ n m k
  rewrite *-commut (n + m) k
  rewrite *-left-distrib-+ k n m
  rewrite *-commut k n
  rewrite *-commut k m = refl

*-assoc : (n m k : â„•) â†’ (n * m) * k â‰¡ n * (m * k)
*-assoc zero m k = refl
*-assoc (suc n) m k =
  begin
    (suc n * m) * k
  âˆ¼âŸ¨âŸ©
    (m + n * m) * k
  âˆ¼âŸ¨ *-right-distrib-+ m (n * m) k âŸ©
    m * k + (n * m) * k
  âˆ¼âŸ¨ cong (m * k +_) (*-assoc n m k) âŸ©
    suc n * m * k
  âˆ
